Java/src/Java/Logic/AssertionLogic.v
@@ -9,6 +9,9 @@ Require Import MapInterface MapFacts.
 Require Import Open Stack Lang OpenILogic Pure ILEmbed PureInsts.
 Require Import UUSepAlg SepAlgInsts HeapArr.
 
+Require Import ExtLib.Core.RelDec.
+Require Import ExtLib.Data.String.
+
 Local Existing Instance ILPre_Ops.
 Local Existing Instance ILPre_ILogic.
 
@@ -42,12 +45,14 @@ Definition heap_add_ptr (h : heap) (p : ptr) (f : field) (v : val) : heap :=
 Definition heap_add_arr (h : heap) (n m : nat) (v : val) : heap :=
   (fst h, add (n, m) v (snd h)).
 
+
 Instance RelHeapPtr : Rel heap_ptr := _.
 Instance PreorderHeapPtr : PreOrder (@rel heap_ptr RelHeapPtr) := _.
 Instance HeapPtrSepAlgOps : SepAlgOps heap_ptr := _.
 Instance SepAlgHeapPtr : SepAlg heap_ptr := _.
 Instance UUSepAlgHeapPtr : UUSepAlg heap_ptr := _.
 
+(*
 Instance SepAlgArrPtr : SepAlg heap_arr := _.
 
 
@@ -56,44 +61,17 @@ Instance PreorderHeap : PreOrder (@rel heap RelHeap) := _.
 Instance HeapSepAlgOps : SepAlgOps heap := _.
 Instance SepAlgHeap : SepAlg heap := _.
 Instance UUSepAlgHeap : UUSepAlg heap := _.
-
-Definition asn1 := ILPreFrm (@rel heap subheap) Prop.
-Instance ILogicOpsAsn1 : ILogicOps asn1 := _.
-Instance ILogicAsn1 : ILogic asn1 := _.
-
-
-Definition asn2 := ILPreFrm ge asn1.
-Instance ILogicOpsAsn2 : ILogicOps asn2 := _.
-Instance ILogicAsn2 : ILogic asn2 := _.
-
-Definition asn := ILPreFrm Prog_wf_sub asn2.
-Instance ILogicOpsAsn : ILogicOps asn := _.
-Instance ILogicAsn : ILogic asn := _.
-
-
-Instance BILOperatorsAsn1 : BILOperators asn1. Admitted.
-Instance BILOperatorsAsn2 : BILOperators asn2. Admitted.
-Instance BILOperatorsAsn : BILOperators asn. Admitted.
-(*Instance BILOperatorsAsn1 : BILOperators asn1 := _. This will work in Coq 8.5
-Instance BILOperatorsAsn2 : BILOperators asn2 := _.
-Instance BILOperatorsAsn : BILOperators asn := _.*)
-
-Instance BILogicAsn1 : BILogic asn1. Admitted.
-Instance BILogicAsn2 : BILogic asn2. Admitted. 
-Instance BILogicAsn  : BILogic asn. Admitted.
-
-Instance IBILogicAsn1 : IBILogic asn1. Admitted.
-Instance IBILogicAsn2 : IBILogic asn2. Admitted.
-Instance IBILogicAsn  : IBILogic asn. Admitted.
- (*
-Instance BILogicAsn1 : BILogic asn1 := _.
-Instance BILogicAsn2 : BILogic asn2 := _.
-Instance BILogicAsn  : BILogic asn := _.
-
-Instance IBILogicAsn1 : IBILogic asn1 := _.
-Instance IBILogicAsn2 : IBILogic asn2 := _.
-Instance IBILogicAsn  : IBILogic asn := _.
 *)
+
+Instance HeapSepAlgOps : SepAlgOps heap := _.
+Instance UUSepAlgHeap : UUSepAlg heap := _.
+
+Definition asn := ILPreFrm Prog_sub (ILPreFrm ge (ILPreFrm (@rel heap subheap) Prop)).
+
+Instance ILogicOpsAsn : ILogicOps asn := _.
+Instance BILogicOpsAsn : BILOperators asn. Admitted.
+Instance BILogicAsn : IBILogic asn. Admitted.
+
 Local Existing Instance EmbedILPreDropOp.
 Local Existing Instance EmbedILPreDrop.
 Local Existing Instance EmbedOpPropProp.
@@ -102,11 +80,12 @@ Local Existing Instance EmbedPropProp.
 Instance EmbedAsnPropOp : EmbedOp Prop asn := _.
 Instance EmbedAsnProp : Embed Prop asn := _.
 
-Definition sasn := @open var _ asn.
+Instance RelDec_var : RelDec (@eq var) := _.
 
-Instance ILOpsSAsn : ILogicOps sasn := _.
-Instance ILogicSAsn : ILogic sasn := _.
-Instance BILOperatorsSAsn : BILOperators sasn := _.
+Definition sasn := (Stack.stack var val) -> asn.
+
+Instance ILogicOpsSAsn : ILogicOps sasn := _.
+Instance BILogicOpsSAsn : BILOperators sasn := _.
 Instance BILogicSAsn : IBILogic sasn := _.
 
 Local Existing Instance EmbedILFunDropOp.
@@ -125,10 +104,6 @@ Instance EmbedSasnPure : Embed vlogic sasn := _.
 
 Require Import SpecLogic.
 
-Instance EmbedAsn1PropOp : EmbedOp Prop asn1 := _.
-Instance EmbedAsn1Prop   : Embed Prop asn1 := _.
-Instance EmbedAsn2SpecOp : EmbedOp spec1 asn2 := _.
-Instance EmbedAsn2Spec   : Embed spec1 asn2 := _.
 Instance EmbedAsnSpecOp  : EmbedOp spec asn := _.
 Instance EmbedAsnSpec    : Embed spec asn := _.
 Instance EmbedSAsnSpecOp : EmbedOp spec sasn := _.
@@ -167,9 +142,9 @@ Instance pure_spec (p : spec) : pure (@embed spec sasn _ p) := _.
 
 Local Transparent ILPre_Ops.
 
-Definition mk_asn (f: Prog_wf -> nat -> heap -> Prop)
+Definition mk_asn (f: Program -> nat -> heap -> Prop)
   (Hnat: forall P k h, f P (S k) h -> f P k h)
-  (HProg: forall P P' k h, Prog_wf_sub P P' -> f P k h -> f P' k h)
+  (HProg: forall P P' k h, Prog_sub P P' -> f P k h -> f P' k h)
   (Hheap: forall P k h h', subheap h h' -> f P k h -> f P k h') : asn.
   refine (mkILPreFrm (fun P => mkILPreFrm (fun k => mkILPreFrm (fun h => f P k h) _) _) _).
 Proof.
@@ -185,7 +160,7 @@ Grab Existential Variables.
 Defined.
 
 Program Definition pointsto_aux (x : ptr) (f : field) (v : val) : asn :=
-  mk_asn (fun P k h => subheap ((empty val) [(x, f) <- v]) (fst h)) _ _ _.
+  mk_asn (fun P k h => subheap (add (x, f) v (empty val)) (fst h)) _ _ _.
 Next Obligation.
   destruct h, h'; simpl in *.
   apply subheap_prod in H as [H _].
@@ -222,8 +197,6 @@ Fixpoint pointsto_arr_aux (x : val) (n : nat) (vs : list val) : asn :=
     | v::vs => pointsto_arr_element x (vint (Z_of_nat n)) v ** 
                                     pointsto_arr_aux x (S n) vs
   end.
-
-Opaque ILogicOpsAsn.
 
 Lemma firstn_nil {A : Type} (n : nat) : firstn n (@nil A) = nil.
 Proof.
