Java/src/Java/Logic/SpecLogic.v
@@ -1,31 +1,30 @@
 Require Import Later Program ILogic ILEmbed ILInsts.
 
+(*
 Local Existing Instance ILLaterNat.
 Local Existing Instance ILLaterNatOps.
 Local Existing Instance ILLaterPre.
 Local Existing Instance ILLaterPreOps.
 Local Existing Instance ILPre_Ops.
 Local Existing Instance ILPre_ILogic.
+*)
 
-Definition spec1 := ILPreFrm ge Prop.
-Definition spec := ILPreFrm Prog_wf_sub spec1.
+Definition spec := ILPreFrm Prog_sub (ILPreFrm ge Prop).
 
-Global Instance ILLOperatorsSpec1 : ILLOperators spec1 := _.
-Global Instance ILogicOpsSpec1 : ILogicOps spec1 := _. 
-Global Instance ILSpec1 : ILLater spec1 := _.
-
+(*
 Global Instance ILLOperatorsSpec : ILLOperators spec := _.
 Global Instance ILogicOpsSpec : ILogicOps spec := _. 
 Global Instance ILSpec : ILLater spec := _.
+*)
 
 Local Transparent ILPre_Ops.
 Require Import Compare_dec.
-Definition mk_spec (f: Prog_wf -> nat -> Prop)
+Definition mk_spec (f: Program -> nat -> Prop)
   (Hnat: forall k P, f P (S k) -> f P k)
-  (HSPred: forall k P P', Prog_wf_sub P P' -> f P k -> f P' k) : spec.
+  (HSPred: forall k P P', Prog_sub P P' -> f P k -> f P' k) : spec.
   refine (mkILPreFrm (fun k => mkILPreFrm (f k) _) _).
 Proof.
-  assert (forall k P P', Prog_wf_sub P P' -> f P k -> f P' k) as HProg.
+  assert (forall k P P', Prog_sub P P' -> f P k -> f P' k) as HProg.
   intros k P P' HPP' S'. eapply HSPred; eassumption. 
   intros p p' Hp'' n S'; simpl in *. eapply HProg; eassumption.
   Grab Existential Variables.
@@ -36,8 +35,8 @@ Proof.
     * subst. apply S'.
 Defined.
 
-Program Definition prog_spec (X : Prog_wf -> Prop) : spec :=
-  mk_spec (fun (P : Prog_wf) _ => forall (Q : Prog_wf) , Prog_wf_sub P Q -> X Q) _ _.
+Program Definition prog_spec (X : Program -> Prop) : spec :=
+  mk_spec (fun (P : Program) _ => forall (Q : Program) , Prog_sub P Q -> X Q /\ valid_program Q = true) _ _.
 Next Obligation.
   intros; apply H0; etransitivity; eassumption.
 Qed.
@@ -54,9 +53,9 @@ Instance EmbedPropSpec : Embed Prop spec := _.
 
 Definition prog_eq Prog : spec := [prog] (fun P => P = Prog).
 
-Lemma prog_eq_to_prop P (f : Prog_wf -> Prop) (H : f P) : prog_eq P |-- [prog] f.
+Lemma prog_eq_to_prop P (f : Program -> Prop) (H : f P) : prog_eq P |-- [prog] f.
 Proof.
   intros Q n HQ R HQR.
   specialize (HQ _ HQR).
-  simpl in *. subst. apply H.
+  simpl in *. subst. intuition congruence.
 Qed.
