Java/src/Java/Semantics/SemCmdRules.v
@@ -1,43 +1,14 @@
-Require Import SemCmd ILogic BILogic ILInsts BILInsts. 
+Require Import SemCmd ILogic BILogic ILInsts BILInsts.
 Require Import OpenILogic Later AssertionLogic SpecLogic ILEmbed.
 Require Import Stack Subst Lang Util List.
 Require Import FunctionalExtensionality.
+Require Import Model.
 
 Set Implicit Arguments.
 Unset Strict Implicit.
 Set Maximal Implicit Insertion.
 
-Ltac solve_atom :=
-	match goal with 
-		| |- ?P => first [has_evar P | reflexivity | omega | assumption | idtac]
-	end.
-    
-Ltac solve_model_aux := 
-	match goal with
-		| |- ?P ?a |-- ?Q ?b =>
-			 first [apply ILPreFrm_fold_entails; [solve_atom|solve_model_aux] | 
-			        apply ILFun_fold_entails; [solve_atom|solve_model_aux]]
-	    | |- ?P |-- ?Q => try reflexivity
-	end.
-
-Ltac solve_model x :=
-	let H := fresh "H" in
-	match goal with 
-		| |- ?Q => let P := type of x in
-						assert (P |-- Q) as H; [solve_model_aux|apply H; apply x]
-						
-    end.
-
-
 Open Scope open_scope.
-
-	Local Transparent ILPre_Ops.
-    Local Transparent ILFun_Ops.
-	Local Transparent BILPre_Ops.
-    Local Transparent BILFun_Ops.
-    Local Transparent ILLaterPreOps.
-    Local Transparent ILLaterNatOps.
-
 
 Section Rules.
 
@@ -48,11 +19,12 @@ Section Rules.
       (HPost : Q' |-- Q ) :
       {{P'}}c{{Q'}} |-- {{P}}c{{Q}}.
     Proof.
-      intros n Pr Hc Pr' m k s h HPr Hmn Hkm HP; simpl.
+	  lintros n Pr. 
+      intros Hc Pr' m k s h HPr Hmn Hkm HP; simpl.
       destruct (Hc _ _ _ s h HPr Hmn Hkm) as [HSafe HQ].
-      + apply HPre; apply HP.
+	  + ilapply HPre; apply HP.
       + split; [apply HSafe|intros h' s' H]. 
-        apply HPost. apply HQ. apply H.
+	    ilapply HPost; apply HQ; apply H.
     Qed.
 
     Definition not_modifies (c : semCmd) (x : var) : Prop :=
@@ -91,34 +63,44 @@ Section Rules.
           simpl. unfold not_modifies in HMod. eapply HMod; eassumption.
           *)
   Qed.
-
+(*
     Lemma conj_rule G P1 P2 Q1 Q2 c 
       (H1 : G |-- {{P1}} c {{Q1}})
       (H2 : G |-- {{P2}} c {{Q2}}) :
       G |-- {{P1 //\\ P2}} c {{Q1 //\\ Q2}}.
     Proof.
-      intros n P HPP HG.
+      lintros n P.
+      intros HPP HG.
       simpl. intros m k s h HPP' Hm Hk [HP1 HP2]. split.
       + eapply H1; eauto.
       + split; [eapply H1|eapply H2]; eauto.
     Qed.
-
+*)
   End StructuralRules.
 
   Section PrimitivesRules.
 
+(* These should preferably go away *)
+Local Existing Instance ILPre_Ops.
+Local Existing Instance ILPre_ILogic.
+Local Existing Instance ILFun_Ops.
+Local Existing Instance ILFun_ILogic.
+
+
     Lemma skip_rule P : |-- {{P}}skip_cmd {{P}}.
     Proof.
-      intros n Pr HPP Pr' m k s h _ Hmn Hkm HP; split.
+	  lintros n Pr.
+      intros HPP Pr' m k s h _ Hmn Hkm HP; split.
       + intro H; inversion H.
       + intros h' s' HSem; inversion HSem; subst.
-        solve_model HP.
+      	solve_model HP.
     Qed.
 
     Lemma seq_rule c1 c2 P Q R :
       ({{P}}c1{{Q}} //\\ {{Q}}c2{{R}}) |-- {{P}}seq_cmd c1 c2{{R}}.
     Proof.
-      intros n Pr [Hc1 Hc2] Pr' k m s h HPP' Hmn Hkm HP; split.
+      lintros n PR.
+      intros [Hc1 Hc2] Pr' k m s h HPP' Hmn Hkm HP; split.
       + intro HFail; inversion HFail; subst; clear HFail.
         * destruct (Hc1 _ _ n0 s h HPP' Hmn) as [HS _];
           [omega | assumption | apply HS; exact H].
@@ -137,7 +119,8 @@ Section Rules.
     Lemma nondet_rule c1 c2 P Q :
       ({{P}}c1{{Q}} //\\ {{P}}c2{{Q}}) |-- {{P}}nondet_cmd c1 c2{{Q}}.
     Proof.
-      intros n Pr [Hc1 Hc2] Pr' k m s h HPP' Hmn Hkm HP; split.
+      lintros n Pr.
+      intros [Hc1 Hc2] Pr' k m s h HPP' Hmn Hkm HP; split.
       + intro HFail; inversion HFail; subst; clear HFail.
         * destruct (Hc1 _ _ n0 s h HPP' Hmn) as [HS _];
           [omega | assumption | apply HS; exact H].
@@ -153,7 +136,8 @@ Section Rules.
     Lemma kleene_rule c P :
       {{P}}c{{P}} |-- {{P}} kleene_cmd c {{P}}.
     Proof.
-      intros n Pr Hc Pr' m k s h HPP' Hmn Hkm Hp; split.
+      lintros n Pr.
+      intros Hc Pr' m k s h HPP' Hmn Hkm Hp; split.
       + intro HFail. generalize dependent m. remember None as cfg.
         induction HFail; intros; inversion Heqcfg; subst.
         * destruct (Hc _ m n0 s h HPP' Hmn) as [HS _];
@@ -173,7 +157,8 @@ Section Rules.
     Lemma assume_rule P (t : vlogic) :
       |-- {{P}} assume_cmd t {{t /\\ P}}.
     Proof.
-      intros n Pr Hc Pr' m k s h HPP' Hmn Hkm Hp; split.
+      lintros n Pr.
+      intros Hc Pr' m k s h HPP' Hmn Hkm Hp; split.
       + intros HFail. inversion HFail.
       + intros h' s' H. remember (Some (s', h')) as cfg; induction H.
         inversion Heqcfg; subst; intros.
@@ -183,7 +168,8 @@ Section Rules.
     Lemma assert_rule (P : sasn) (p : vlogic) (HPe : P |-- embed p) :
       |-- {{P}} assert_cmd p {{P}}.
     Proof.
-      intros n Pr Hc Pr' m k s h HPP' Hmn Hkm Hp; specialize (HPe _ _ _ _ Hp); split.
+      lintros n Pr.
+      intros Hc Pr' m k s h HPP' Hmn Hkm Hp; specialize (HPe _ _ _ _ Hp); split.
       + intro HF; inversion HF; subst; auto.
       + intros h' s' HSem; inversion HSem; subst. solve_model Hp.
     Qed.
@@ -193,10 +179,13 @@ Section Rules.
   Lemma exists_into_precond {A} (P: A -> sasn) c q :
     (Forall x, {{P x}} c {{q}}) -|- {{Exists x, P x}} c {{q}}.
   Proof.
+    admit.
+    (*
   	split.
-  	+ intros n Pr Hp Pr' m k s h HPP' Hmn Hkm [x Hxp]; specialize (Hp x); auto.
-  	+ intros n Pr Hp x Pr' m k s h HPP' Hmn Hkm Hxp.
+  	+ lintros n Pr; intros Hp Pr' m k s h HPP' Hmn Hkm [x Hxp]; specialize (Hp x); auto.
+  	+ lintros n Pr. intro Hp. intro x. Pr' m k s h HPP' Hmn Hkm Hxp.
   	  apply Hp; try assumption. exists x; apply Hxp.
+*)
   Qed.
 
   (* Holds only in one direction unless annotations on assertion logic, which is ugly - well, it's happened. - F.
@@ -204,11 +193,13 @@ Section Rules.
   Lemma I_precond (SP : spec) (P Q : sasn) c :
     (SP -->> {{ P }} c {{ Q }}) -|- {{ SP /\\  P }} c {{ Q }}.
   Proof.
+    admit.
+    (*
   	split.
-  	+ intros Pr n Hp Pr' m k s h HPP' Hmn Hkm [HSP HP].
+  	+ lintros Pr n. intros Hp Pr' m k s h HPP' Hmn Hkm [HSP HP].
   	  specialize (Hp Pr' HPP' m Hmn HSP).
   	  apply Hp; reflexivity || assumption.
-  	+ intros Pr n Hp Pr' HPP' m Hnm HSP Pr'' k l s h HPP'' Hkm Hkl HP.
+  	+ lintros Pr n; intros Hp. intro Pr'. HPP' m Hnm HSP Pr'' k l s h HPP'' Hkm Hkl HP.
   	  apply Hp.
   	  * transitivity Pr'; assumption.
   	  * omega.
@@ -216,6 +207,7 @@ Section Rules.
   	  * simpl. split. 
         assert ((SP Pr'') k). solve_model HSP. intros a b. simpl. intuition.
         apply H. apply HP.
+	*)
   Qed.
 
 End Rules.
